Implement key derivation

code/chacha20poly1305/Hacl.Impl.Chacha20Poly1305.Poly.fst
@@ -12,7 +12,57 @@ open FStar.Mul
 
 module Spec = Spec.Chacha20Poly1305
 module Poly = Hacl.Impl.Poly1305
+open Hacl.Impl.Poly1305.Fields
+module ChachaCore = Hacl.Impl.Chacha20.Core32
+module Chacha = Hacl.Impl.Chacha20
 
+#set-options "--z3rlimit 20 --max_fuel 0 --max_ifuel 1"
+
+val derive_key:
+  k:lbuffer uint8 32ul ->
+  n:lbuffer uint8 12ul ->
+  out:lbuffer uint8 64ul ->
+  Stack unit
+    (requires fun h -> live h k /\ live h out /\ live h n /\
+      disjoint k out /\ disjoint n out)
+    (ensures fun h0 _ h1 -> modifies (loc out) h0 h1 /\
+      Seq.equal
+        (as_seq h1 out)
+        (Spec.Chacha20.chacha20_key_block0 (as_seq h0 k) (as_seq h0 n))
+    )
+
+let derive_key k n out =
+  push_frame();
+  let ctx = ChachaCore.create_state () in
+  Chacha.chacha20_init ctx k n 0ul;
+  ChachaCore.store_state out ctx;
+  pop_frame()
+  
+// Implements the actual poly1305_do operation
+val poly1305_do_core:
+  s:field_spec ->         // Needed for the vectorized operation
+  k:lbuffer uint8 32ul -> // key
+  aadlen:size_t ->
+  aad:lbuffer uint8 aadlen -> // authenticated additional data  
+  (mlen:size_t{v mlen + 16 <= max_size_t /\ v aadlen + v mlen / 64 <= max_size_t}) ->
+  m:lbuffer uint8 mlen -> // plaintext
+  out:lbuffer uint8 16ul -> // output: tag
+  Stack unit
+    (requires fun h ->
+      live h k /\ live h aad /\ live h m /\ live h out)
+    (ensures (fun h0 _ h1 -> modifies (loc out) h0 h1 /\
+      as_seq h1 out == Spec.poly1305_do (as_seq h0 k) (v mlen) (as_seq h0 m) (v aadlen) (as_seq h0 aad)))
+
+let poly1305_do_core s k aadlen aad mlen m out =
+  push_frame();
+  let ctx = create (nlimb s +. precomplen s) (limb_zero s) in
+  Poly.poly1305_init ctx k;
+  let block = create 16ul (u8 0) in
+  // TODO: Padding should go here
+  admit();
+  pop_frame()
+
+// Derives the key, and then perform poly1305
 val poly1305_do:
   k:lbuffer uint8 32ul ->
   n:lbuffer uint8 12ul ->
@@ -23,9 +73,19 @@ val poly1305_do:
   out:lbuffer uint8 16ul ->
   Stack unit
     (requires (fun h ->
-      live h k /\ live h aad /\ live h m /\ live h out))
+      live h k /\ live h n /\ live h aad /\ live h m /\ live h out))
     (ensures (fun h0 _ h1 -> modifies (loc out) h0 h1 /\ (
       let poly_k = Seq.sub (Spec.Chacha20.chacha20_key_block0 (as_seq h0 k) (as_seq h0 n)) 0 32 in
       as_seq h1 out == Spec.poly1305_do poly_k (v mlen) (as_seq h0 m) (v aadlen) (as_seq h0 aad))))
 
-let poly1305_do k aadlen aad mlen m out = admit()
+let poly1305_do k n aadlen aad mlen m out =
+  push_frame ();
+  // Create a new buffer to derive the key
+  let tmp = create 64ul (u8 0) in
+  derive_key k n tmp;
+  // The derived key should only be the first 32 bytes
+  let key = sub tmp 0ul 32ul in
+  // M32 can be abstracted away for a vectorized AEAD
+  poly1305_do_core M32 key aadlen aad mlen m out;
+  pop_frame()
+
